theories/run_test.v
@@ -2,6 +2,11 @@ From mathcomp Require Import all_ssreflect.
 From det Require Import lang run.
 Import Language.
 
+
+Notation "X &&& Y" := (And X _ Y) (at level 3).
+Notation "X ||[ Y s ]" := (Or X s Y) (at level 3).
+Notation "` X" := ((Call X)) (at level 3).
+
 Definition empty_sig : sigT := fun _ => b(d Func).
 
 Definition build_progr l := {|
@@ -10,34 +15,31 @@ Definition build_progr l := {|
     rules := l;
 |}.
 
-(* Module RunAxiom:= Run(UAxioms). *)
-    Definition unifyF    (t1 t2 : Tm) (s : Sigma) :=
-      match t1, t2 with
-      | Code (v X), _ => match s.(sigma) X with None => Some {| sigma := (fun x => if x == X then Some t2 else s.(sigma) x) |} | Some t => if t == t2 then Some s else None end
-      | _, Code (v X) => match s.(sigma) X with None => Some {| sigma := (fun x => if x == X then Some t1 else s.(sigma) x) |} | Some t => if t == t1 then Some s else None end
-      | _, _ => if t1 == t2 then Some s else None
-      end.
+(* Section RunAxiom:= Run(UAxioms). *)
+Definition unifyF    (t1 t2 : Tm) (s : Sigma) :=
+  match t1, t2 with
+  | Code (v X), _ => match s.(sigma) X with None => Some {| sigma := (fun x => if x == X then Some t2 else s.(sigma) x) |} | Some t => if t == t2 then Some s else None end
+  | _, Code (v X) => match s.(sigma) X with None => Some {| sigma := (fun x => if x == X then Some t1 else s.(sigma) x) |} | Some t => if t == t1 then Some s else None end
+  | _, _ => if t1 == t2 then Some s else None
+  end.
 
-    Definition matchingF (t1 t2 : Tm) (s : Sigma) := if t1 == t2 then Some s else None.
-  Definition unif : Unif := {|
-    unify := unifyF;
-    matching := matchingF
-  |}.
-
-Module Test1.
-
-  (* Module U <: Unif. *)
-  (* End U. *)
-
-  (* Module Run := Run(U). *)
-  (* Import Run. *)
+Definition matchingF (t1 t2 : Tm) (s : Sigma) := if t1 == t2 then Some s else None.
+Definition unif : Unif := {|
+  unify := unifyF;
+  matching := matchingF
+|}.
 
 
-  Definition v_X := Code (v 0).
-  Definition pred_q x  := Comb (Code (p 1)) x.
-  Definition pred_p x  := Comb (Code (p 0)) x.
-  Definition pred_r x  := Comb (Code (p 2)) x.
-  Definition pred_fail := Code (p 100).
+Definition v_X := Code (v 0).
+Definition pred_q x  := Comb (Code (p 1)) x.
+Definition pred_p x  := Comb (Code (p 0)) x.
+Definition pred_r x  := Comb (Code (p 2)) x.
+Definition pred_fail := Code (p 100).
+
+Definition s1 := {| sigma := (fun x => if x == 0 then Some (Data 1) else None) |}.
+Definition s2 := {| sigma := (fun x => if x == 0 then Some (Data 2) else None) |}.
+
+Section Test1.
 
   Definition p_test : program := build_progr [:: 
       mkR (pred_p (Data 1)) [::] ;
@@ -46,15 +48,8 @@ Module Test1.
       mkR (pred_q (Data 1)) [:: Call (pred_p v_X) ; Call (pred_r v_X) ] 
     ].
 
-  Notation "X &&& Y" := (And X _ Y) (at level 3).
-  Notation "X ||[ Y s ]" := (Or X s Y) (at level 3).
-  Notation "` X" := (Goal _ (Call X)) (at level 3).
-  (* Notation "[ x -> _]" := {| sigma := (fun x : V => _) |} (x binder). *)
 
-  Definition s1 := {| sigma := (fun x => if x == 0 then Some (Data 1) else None) |}.
-  Definition s2 := {| sigma := (fun x => if x == 0 then Some (Data 2) else None) |}.
-
-  Goal exists r, runb unif empty (Goal p_test (Call (pred_q (Data 1)))) s2 r false.
+  Goal exists r, runb unif empty (CallS p_test (pred_q (Data 1))) s2 r false.
   Proof.
     eexists.
     apply: run_backtrack => //.
@@ -92,27 +87,18 @@ Module Test1.
   Qed.
 End Test1.
 
-Module Test5.
+Section Test5.
 
-  Definition v_X := Code (v 0).
   Definition pred_f x  := Comb (Code (p 1)) x.
   Definition pred_g x  := Comb (Code (p 0)) x.
 
-  Definition p_test : program := build_progr [:: 
+  Definition p_test1 : program := build_progr [:: 
       mkR (pred_f (Data 0)) [:: Call (pred_g v_X); Cut] ;
       mkR (pred_g (Data 1)) [::];
       mkR (pred_g (Data 2)) [::]
     ].
 
-  Notation "X &&& Y" := (And X _ Y) (at level 3).
-  Notation "X ||[ Y s ]" := (Or X s Y) (at level 3).
-  Notation "` X" := (Goal _ (Call X)) (at level 3).
-  (* Notation "[ x -> _]" := {| sigma := (fun x : V => _) |} (x binder). *)
-
-  Definition s1 := {| sigma := (fun x => if x == 0 then Some (Data 1) else None) |}.
-  Definition s2 := {| sigma := (fun x => if x == 0 then Some (Data 2) else None) |}.
-
-  Goal exists r, runb unif empty (Goal p_test (Call (pred_f (Data 0)))) s1 r false /\ next_alt None r = None.
+  Goal exists r, runb unif empty (CallS p_test1 ((pred_f (Data 0)))) s1 r false /\ next_alt None r = None.
   Proof.
     repeat eexists.
     apply: run_backtrack.
@@ -131,7 +117,7 @@ Module Test5.
       rewrite -/s1-/s2.
       apply: run_done.
       apply: expanded_step => //.
-      rewrite [Cut]lock.
+      rewrite [CutS]lock.
       apply: expanded_step => //=.
       rewrite -lock [mkAnd]lock /= -/s1 -/s2.
       rewrite -lock [mkOr]lock /=.
@@ -144,29 +130,20 @@ Module Test5.
   Qed.
 End Test5.
 
-Module Test6.
+Section Test6.
 
-  Definition v_X := Code (v 0).
-  Definition pred_f x  := Comb (Code (p 1)) x.
-  Definition pred_g x  := Comb (Code (p 0)) x.
   Definition pred_true := (Code (p 0)).
 
-  Definition p_test : program := build_progr [:: 
+  Definition p_test2 : program := build_progr [:: 
       mkR pred_true [::];
       mkR (pred_f (Data 0)) [:: Call (pred_g v_X); Call pred_true; Cut] ;
       mkR (pred_g (Data 1)) [::];
       mkR (pred_g (Data 2)) [::]
   ].
 
-  Notation "X &&& Y" := (And X _ Y) (at level 3).
-  Notation "X ||[ Y s ]" := (Or X s Y) (at level 3).
-  Notation "` X" := (Goal _ (Call X)) (at level 3).
   (* Notation "[ x -> _]" := {| sigma := (fun x : V => _) |} (x binder). *)
 
-  Definition s1 := {| sigma := (fun x => if x == 0 then Some (Data 1) else None) |}.
-  Definition s2 := {| sigma := (fun x => if x == 0 then Some (Data 2) else None) |}.
-
-  Goal exists r, runb unif empty (Goal p_test (Call (pred_f (Data 0)))) s1 r false /\ next_alt None r = None.
+  Goal exists r, runb unif empty (CallS p_test2 ((pred_f (Data 0)))) s1 r false /\ next_alt None r = None.
   Proof.
     repeat eexists.
     apply: run_backtrack.
@@ -203,12 +180,11 @@ Module Test6.
 End Test6.
 
 
-Module Test2.
+Section Test2.
   (* Import RunAxiom. *)
   Goal expand unif empty (Or OK empty OK) = Success empty (Or OK empty OK) . by []. Qed.
 
-  Goal forall p, runb unif empty (Or (Goal p Cut) empty OK) empty (Or Bot empty Bot) false.
-    move=> pr //=.
+  Goal runb unif empty (Or (CutS) empty OK) empty (Or Bot empty Bot) false.
     apply: run_done => //=. 
     apply: expanded_step => //=.
     by apply: expanded_done => /=.
@@ -216,9 +192,9 @@ Module Test2.
     reflexivity. 
   Qed.
 
-  Goal forall p r, 
-    runb unif empty (Or (Goal p Cut) empty r) empty (Or Bot empty (cutr r)) false.
-    move=> p r.
+  Goal forall r, 
+    runb unif empty (Or (CutS) empty r) empty (Or Bot empty (cutr r)) false.
+    move=> r.
     apply: run_done.
     apply: expanded_step => //=.
     apply: expanded_done => //=.
@@ -232,7 +208,7 @@ Module Test2.
     reflexivity. Qed.
 
   (* (Dead \/ !) \/ C *)
-  Goal expand unif empty (Or (Or Dead empty (Goal (build_progr [::]) Cut)) empty Top) = Expanded empty (Or (Or Dead empty OK) empty Top) .
+  Goal expand unif empty (Or (Or Dead empty (CutS)) empty Top) = Expanded empty (Or (Or Dead empty OK) empty Top) .
   Proof.
     move=>//=.
   Qed.
